before hhs

src/computational_monads/query_tracking/query_count/generate.lean
@@ -29,7 +29,7 @@ def generate_aux (qc : spec.query_count)
   (oa : Π (i : spec.ι), oracle_comp spec' (τ i)) :
   list spec.ι → oracle_comp spec' (spec.indexed_list τ)
 | (j :: js) :=
-  do {ts ← vector.to_list <$> repeat (oa j) (qc.get_count j),
+  do {ts ← repeat (oa j) (qc.get_count j),
       (+) (of_list ts) <$> generate_aux js}
 | [] := return ∅
 
@@ -38,24 +38,24 @@ variables (qc : spec.query_count) (oa : Π (i : spec.ι), oracle_comp spec' (τ 
 @[simp] lemma generate_aux_nil : generate_aux qc oa [] = return ∅ := rfl
 
 lemma generate_aux_cons (j js) : generate_aux qc oa (j :: js) =
-  vector.to_list <$> repeat (oa j) (qc.get_count j) >>= λ ts,
+  repeat (oa j) (qc.get_count j) >>= λ ts,
     ((+) (of_list ts)) <$> generate_aux qc oa js := by rw [generate_aux]
 
 lemma generate_aux_cons' (j js) : generate_aux qc oa (j :: js) =
-  ((+) <$> of_list <$> vector.to_list <$> repeat (oa j) (qc.get_count j))
+  ((+) <$> of_list <$> repeat (oa j) (qc.get_count j))
     <*> (generate_aux qc oa js) :=
 by simp [generate_aux, map_eq_bind_pure_comp, seq_eq_bind_map, bind_assoc]
 
 @[simp] lemma generate_aux_singleton (j : spec.ι) : generate_aux qc oa [j] =
-  of_list <$> vector.to_list <$> repeat (oa j) (qc.get_count j) :=
+  of_list <$> repeat (oa j) (qc.get_count j) :=
 by simpa only [generate_aux, map_return, add_empty]
 
 @[simp] lemma generate_aux_empty (js : list spec.ι) : generate_aux ∅ oa js = return ∅ :=
 begin
   induction js with j js hjs,
   { refl },
-  { rw [generate_aux_cons, get_count_empty, repeat_zero, map_return, oracle_comp.return_bind,
-      vector.to_list_nil, of_list_nil, empty_add_eq_id, id_map, hjs] }
+  { rw [generate_aux_cons, get_count_empty, repeat_zero, oracle_comp.return_bind,
+      of_list_nil, empty_add_eq_id, id_map, hjs] }
 end
 
 lemma generate_aux_eq_generate_aux_filter (js : list spec.ι) : generate_aux qc oa js =
@@ -66,7 +66,7 @@ begin
   { by_cases hj : (∈ qc.active_oracles) j,
     { simp_rw [list.filter, hj, if_true, generate_aux_cons, hjs] },
     { simp_rw [list.filter, hj, if_false, generate_aux_cons],
-      rw [get_count_eq_zero qc hj, repeat_zero, map_return, vector.to_list_nil,
+      rw [get_count_eq_zero qc hj, repeat_zero,
         oracle_comp.return_bind, of_list_nil, empty_add_eq_id, id_map, hjs] } }
 end
 
@@ -85,19 +85,16 @@ end
 -- end
 
 @[simp] lemma generate_aux_of_nat (js : list spec.ι) (j n) : generate_aux (of_nat j n) oa js =
-  of_list <$> vector.to_list <$> repeat (oa j) (n * js.count j) :=
+  of_list <$> repeat (oa j) (n * js.count j) :=
 begin
   induction js with j' js hjs,
-  { rw [generate_aux_nil, list.count_nil, mul_zero, repeat_zero, map_return, map_return,
-      of_list_vector_to_list_nil] },
+  { rw [generate_aux_nil, list.count_nil, mul_zero, repeat_zero, map_return, of_list_nil] },
   { by_cases hj : j = j',
     { induction hj,
       rw [generate_aux_cons, get_count_of_nat_self, list.count_cons_self, mul_add,
         mul_one, add_comm, hjs],
       simp only [map_eq_bind_pure_comp, bind_assoc, seq_eq_bind_map, function.comp_app,
-        pure_bind, vector.to_list_append, of_list_append],
-      
-         },
+        pure_bind, vector.to_list_append, of_list_append, repeat_add] },
     { rw [generate_aux_cons, get_count_of_nat, if_neg hj, repeat_zero, list.count_cons_of_ne hj],
       simp only [hjs, map_pure, vector.to_list_empty, map_map_eq_map_comp, pure_bind, of_list_nil,
         empty_add_eq_id, function.comp.left_id] } }
@@ -158,7 +155,8 @@ begin
     simp_rw [list.mem_cons_iff, sep_or_eq_sup, ← h, ← htsil, to_query_count_add],
     refine trans _ (sup_eq_add _ _ _).symm,
     { rw [to_query_count_of_list, sep_index_eq, add_left_inj, of_nat, apply_eq_replicate_get_count,
-        of_list_inj, list.replicate_left_inj, vector.to_list_length] },
+        of_list_inj, list.replicate_left_inj],
+      exact hts.1 },
     { suffices : j ∉ il'.active_oracles,
       by by_cases hj : j ∈ qc.active_oracles; simp [hj, this],
       have : il'.active_oracles = qc.active_oracles.filter (∈ js),
@@ -254,10 +252,10 @@ by simp only [generate, active_oracles_empty, finset.to_list_empty, generate_aux
 @[simp] lemma generate_zero : generate 0 oa = return 0 := generate_empty oa
 
 @[simp] lemma generate_of_nat (i n) : generate (of_nat i n) oa =
-  of_list <$> vector.to_list <$> repeat (oa i) n :=
+  of_list <$> repeat (oa i) n :=
 begin
   cases n with n,
-  simp_rw [of_nat_zero, generate_empty, repeat_zero, map_pure, vector.to_list_empty, of_list_nil],
+  simp_rw [of_nat_zero, generate_empty, repeat_zero, map_pure, of_list_nil],
   rw [generate, generate_aux_of_nat, finset.count_to_list, active_oracles_of_nat,
     if_neg (nat.succ_ne_zero n)],
   congr; simp only [finset.mem_singleton, eq_self_iff_true, if_true, mul_one]
@@ -338,8 +336,7 @@ begin
 end
 
 @[pairwise_dist_equiv] lemma generate_increment_dist_equiv (i : spec.ι) (n : ℕ) :
-  generate (qc.increment i n) oa ≃ₚ
-    (+) <$> (of_list <$> vector.to_list <$> repeat (oa i) n) <*> generate qc oa :=
+  generate (qc.increment i n) oa ≃ₚ (+) <$> (of_list <$> repeat (oa i) n) <*> generate qc oa :=
 begin
   rw [increment_eq_of_nat_add],
   rw_dist_equiv [generate_add_dist_equiv],
