src/crypto_constructions/one_time_pad.lean
@@ -20,7 +20,7 @@ open oracle_comp oracle_spec
 
 noncomputable def one_time_pad (n : ℕ) :
   symm_enc_alg (vector bool n) (vector bool n) (vector bool n) :=
-{ keygen := λ _, oracle_comp.repeat coin n,
+{ keygen := λ _, $ᵗ (vector bool n), -- random bit-string
   encrypt := λ ⟨m, k⟩, vector.zip_with bxor m k,
   decrypt := λ ⟨c, k⟩, vector.zip_with bxor c k,
   complete := λ m k _, (vector.ext (λ i, by simp [vector.zip_with_nth]) :
@@ -31,7 +31,7 @@ namespace one_time_pad
 variables {n : ℕ}
 
 @[simp] lemma keygen_apply (u : unit) :
-  (one_time_pad n).keygen u = oracle_comp.repeat coin n := rfl
+  (one_time_pad n).keygen u = $ᵗ (vector bool n) := rfl
 
 @[simp] lemma encrypt_apply (m k : vector bool n) :
   (one_time_pad n).encrypt (m, k) = m.zip_with bxor k := rfl
@@ -39,25 +39,12 @@ variables {n : ℕ}
 @[simp] lemma decrypt_apply (c k : vector bool n) :
   (one_time_pad n).decrypt (c, k) = c.zip_with bxor k := rfl
 
-theorem perfect_secrecy (n : ℕ) : (one_time_pad n).perfect_secrecy :=
-begin
-  refine ((one_time_pad n).perfect_secrecy_iff_of_equal_card rfl rfl).2 ⟨λ v, _, λ m c, _⟩,
-  { calc ⁅= v | (one_time_pad n).keygen ()⁆ = (list.map ⁅coin⁆ v.to_list).prod :
-        by rw [keygen_apply, prob_output_repeat, eval_dist_coe_sub_spec]
-      ... = 2⁻¹ ^ (list.map ⁅coin⁆ v.to_list).length :
-        list.prod_eq_pow_card _ 2⁻¹ (λ x hx, let ⟨y, hy⟩ := list.mem_map.1 hx in
-          by simp only [← hy.2, eval_dist_query, pmf.uniform_of_fintype_apply, coin_spec_range,
-            fintype.card_bool, nat.cast_bit0, algebra_map.coe_one])
-      ... = (fintype.card (vector bool n))⁻¹ : by simp_rw [card_vector, fintype.card_bool,
-        nat.cast_pow, nat.cast_two, ennreal.inv_pow, list.length_map, vector.to_list_length] },
-  { refine ⟨vector.zip_with bxor m c, ⟨_, _⟩, λ k hk, _⟩,
-    { simp only [keygen_apply, mem_support_repeat_iff_forall, support_coe_sub_spec, coin,
-        support_query, set.top_eq_univ, set.mem_univ, imp_true_iff] },
-    { exact vector.ext (λ i, by simp only [encrypt_apply, vector.zip_with_nth,
-        ← bool.bxor_assoc, bxor_self, bool.bxor_ff_left]) },
-    { exact vector.ext (λ i, by simp only [hk.2.symm, ← bool.bxor_assoc, encrypt_apply,
-        vector.zip_with_nth, bxor_self, bool.bxor_ff_left]) } }
-end
+lemma zip_with_bxor_comm (xs ys zs : vector bool n) :
+  vector.zip_with bxor xs ys = zs ↔ vector.zip_with bxor xs zs = ys :=
+by refine ⟨λ h, _, λ h, _⟩; { rw [← h], ext i, simp [← bool.bxor_assoc] }
 
+theorem perfect_secrecy (n : ℕ) : (one_time_pad n).perfect_secrecy :=
+((one_time_pad n).perfect_secrecy_iff_of_equal_card rfl rfl).2
+  ⟨by simp, λ m c, by simp [zip_with_bxor_comm m _ c]⟩
 
 end one_time_pad
