src/computational_monads/constructions/try_until.lean
@@ -18,189 +18,191 @@ Because this may not always produce a final result, we use an option type to rep
 We implement this as a mapping of `oracle_comp.repeat` for simplicity in deriving lemmas.
 This means that the computation always "runs" `n` times even if a result is found before that.
 However it isn't clear that this is commonly a problem, so we take this approach for now.
+
+TODO: this can be brought back but isn't needed now.
 -/
 
-namespace oracle_comp
+-- namespace oracle_comp
 
-open oracle_spec
+-- open oracle_spec
 
-variables {α β γ : Type} {spec spec' : oracle_spec}
+-- variables {α β γ : Type} {spec spec' : oracle_spec}
 
-/-- Computation that repeats `oa` until `p` holds on the result, with at most `n` attempts. -/
-def try_until (oa : oracle_comp spec α) (p : α → Prop) [decidable_pred p]
-  (n : ℕ) : oracle_comp spec (option α) :=
-(λ xs, (vector.to_list xs).find p) <$> (repeat oa n)
+-- /-- Computation that repeats `oa` until `p` holds on the result, with at most `n` attempts. -/
+-- def try_until (oa : oracle_comp spec α) (p : α → Prop) [decidable_pred p]
+--   (n : ℕ) : oracle_comp spec (option α) :=
+-- (λ xs, (vector.to_list xs).find p) <$> (repeat oa n)
 
-variables (oa : oracle_comp spec α) (p : α → Prop) [decidable_pred p]
-  (n : ℕ) {m : ℕ} (x : option α)
+-- variables (oa : oracle_comp spec α) (p : α → Prop) [decidable_pred p]
+--   (n : ℕ) {m : ℕ} (x : option α)
 
-lemma try_until_zero : oa.try_until p 0 =
-  (λ xs, (vector.to_list xs).find p) <$> (return vector.nil) := rfl
+-- lemma try_until_zero : oa.try_until p 0 =
+--   (λ xs, (vector.to_list xs).find p) <$> (return vector.nil) := rfl
 
-lemma try_until_succ : oa.try_until p n.succ =
-  (λ xs, (vector.to_list xs).find p) <$> do {a ← oa, as ← oa.repeat n, return (a ::ᵥ as)} :=
-by rw [try_until, repeat_succ, seq_map_eq_bind_bind]
+-- lemma try_until_succ : oa.try_until p n.succ =
+--   (λ xs, (vector.to_list xs).find p) <$> do {a ← oa, as ← oa.repeat n, return (a ::ᵥ as)} :=
+-- by rw [try_until, repeat_succ, seq_map_eq_bind_bind]
 
-/-- Any positive result of `oa.try_until p n` will be some output of `oa`. -/
-lemma mem_support_of_some_mem_support_try_until {x : α}
-  (hx : some x ∈ (oa.try_until p m).support) : x ∈ oa.support :=
-begin
-  simp_rw [try_until, support_map, set.mem_image, mem_support_repeat_iff_forall] at hx,
-  exact let ⟨xs, hxs, hxs'⟩ := hx in hxs x (list.find_mem hxs')
-end
+-- /-- Any positive result of `oa.try_until p n` will be some output of `oa`. -/
+-- lemma mem_support_of_some_mem_support_try_until {x : α}
+--   (hx : some x ∈ (oa.try_until p m).support) : x ∈ oa.support :=
+-- begin
+--   simp_rw [try_until, support_map, set.mem_image, mem_support_repeat_iff_forall] at hx,
+--   exact let ⟨xs, hxs, hxs'⟩ := hx in hxs x (list.find_mem hxs')
+-- end
 
-/-- Any positive result of `oa.try_until p n` will satisfy the predicate `p`. -/
-lemma pos_of_some_mem_support_try_until {x : α}
-  (hx : some x ∈ (oa.try_until p m).support) : p x :=
-begin
-  simp_rw [try_until, support_map, set.mem_image, mem_support_repeat_iff_forall] at hx,
-  exact let ⟨xs, hxs, hxs'⟩ := hx in list.find_some hxs'
-end
+-- /-- Any positive result of `oa.try_until p n` will satisfy the predicate `p`. -/
+-- lemma pos_of_some_mem_support_try_until {x : α}
+--   (hx : some x ∈ (oa.try_until p m).support) : p x :=
+-- begin
+--   simp_rw [try_until, support_map, set.mem_image, mem_support_repeat_iff_forall] at hx,
+--   exact let ⟨xs, hxs, hxs'⟩ := hx in list.find_some hxs'
+-- end
 
-section try_until_zero
+-- section try_until_zero
 
-/-- Running a computation zero times is distributionally equivalent to just returning failure. -/
-@[pairwise_dist_equiv] lemma try_until_zero_dist_equiv :
-  oa.try_until p 0 ≃ₚ (return none : oracle_comp spec _) :=
-by simp [dist_equiv_return_iff', try_until_zero]
+-- /-- Running a computation zero times is distributionally equivalent to just returning failure. -/
+-- @[pairwise_dist_equiv] lemma try_until_zero_dist_equiv :
+--   oa.try_until p 0 ≃ₚ (return none : oracle_comp spec _) :=
+-- by simp [dist_equiv_return_iff', try_until_zero]
 
-/-- Running a computation zero times will never return a positive result. -/
-@[simp] lemma support_try_until_zero : (oa.try_until p 0).support = {none} :=
-(try_until_zero_dist_equiv oa p).support_eq.trans (support_return _ _)
+-- /-- Running a computation zero times will never return a positive result. -/
+-- @[simp] lemma support_try_until_zero : (oa.try_until p 0).support = {none} :=
+-- (try_until_zero_dist_equiv oa p).support_eq.trans (support_return _ _)
 
-lemma mem_support_try_until_zero_iff : x ∈ (oa.try_until p 0).support ↔ x = none :=
-by rw [support_try_until_zero, set.mem_singleton_iff]
+-- lemma mem_support_try_until_zero_iff : x ∈ (oa.try_until p 0).support ↔ x = none :=
+-- by rw [support_try_until_zero, set.mem_singleton_iff]
 
-@[simp] lemma fin_support_try_until_zero [decidable_eq α] :
-  (oa.try_until p 0).fin_support = {none} :=
-(try_until_zero_dist_equiv oa p).fin_support_eq.trans (fin_support_return _ _)
+-- @[simp] lemma fin_support_try_until_zero [decidable_eq α] :
+--   (oa.try_until p 0).fin_support = {none} :=
+-- (try_until_zero_dist_equiv oa p).fin_support_eq.trans (fin_support_return _ _)
 
-lemma mem_fin_support_try_until_iff [decidable_eq α] :
-  x ∈ (oa.try_until p 0).fin_support ↔ x = none :=
-by rw [fin_support_try_until_zero, finset.mem_singleton]
+-- lemma mem_fin_support_try_until_iff [decidable_eq α] :
+--   x ∈ (oa.try_until p 0).fin_support ↔ x = none :=
+-- by rw [fin_support_try_until_zero, finset.mem_singleton]
 
-@[simp] lemma eval_dist_try_until_zero : ⁅oa.try_until p 0⁆ = pmf.pure none :=
-(try_until_zero_dist_equiv oa p).eval_dist_eq.trans (eval_dist_return _)
+-- @[simp] lemma eval_dist_try_until_zero : ⁅oa.try_until p 0⁆ = pmf.pure none :=
+-- (try_until_zero_dist_equiv oa p).eval_dist_eq.trans (eval_dist_return _)
 
-lemma prob_output_try_until_zero : ⁅= x | oa.try_until p 0⁆ = x.rec_on 1 (λ _, 0) :=
-((try_until_zero_dist_equiv oa p).prob_output_eq x).trans (by cases x; simp)
+-- lemma prob_output_try_until_zero : ⁅= x | oa.try_until p 0⁆ = x.rec_on 1 (λ _, 0) :=
+-- ((try_until_zero_dist_equiv oa p).prob_output_eq x).trans (by cases x; simp)
 
--- @[simp] lemma prob_event_try_until_zero_eq_indicator (q : option α → Prop) :
---   ⁅q | oa.try_until p 0⁆ = e.indicator (λ _, 1) none :=
--- ((try_until_zero_dist_equiv oa p).prob_event_eq e).trans (prob_event_return_eq_indicator spec _ e)
+-- -- @[simp] lemma prob_event_try_until_zero_eq_indicator (q : option α → Prop) :
+-- --   ⁅q | oa.try_until p 0⁆ = e.indicator (λ _, 1) none :=
+-- -- ((try_until_zero_dist_equiv oa p).prob_event_eq e).trans (prob_event_return_eq_indicator spec _ e)
 
-@[simp] lemma prob_event_try_until_zero (q : option α → Prop) [decidable_pred q] :
-  ⁅q | oa.try_until p 0⁆ = if q none then 1 else 0 :=
-((try_until_zero_dist_equiv oa p).prob_event_eq q).trans (prob_event_return spec _ q)
+-- @[simp] lemma prob_event_try_until_zero (q : option α → Prop) [decidable_pred q] :
+--   ⁅q | oa.try_until p 0⁆ = if q none then 1 else 0 :=
+-- ((try_until_zero_dist_equiv oa p).prob_event_eq q).trans (prob_event_return spec _ q)
 
-end try_until_zero
+-- end try_until_zero
 
-section try_until_succ
+-- section try_until_succ
 
-@[pairwise_dist_equiv] lemma try_until_succ_dist_equiv : oa.try_until p n.succ ≃ₚ
-  do {x ← oa, if p x then return (some x) else oa.try_until p n} :=
-begin
-  simp_rw [try_until_succ, map_bind, map_pure],
-  refine bind_dist_equiv_bind_of_dist_equiv_right' _ (λ x, _),
-  by_cases hp : p x,
-  { simp only [hp, vector.to_list_cons, list.find_cons_of_pos, if_true,
-      bind_const_dist_equiv_iff] },
-  { simp only [hp, try_until, map_eq_bind_pure_comp, vector.to_list_cons,
-      list.find_cons_of_neg, not_false_iff, if_false] }
-end
+-- @[pairwise_dist_equiv] lemma try_until_succ_dist_equiv : oa.try_until p n.succ ≃ₚ
+--   do {x ← oa, if p x then return (some x) else oa.try_until p n} :=
+-- begin
+--   simp_rw [try_until_succ, map_bind, map_pure],
+--   refine bind_dist_equiv_bind_of_dist_equiv_right' _ (λ x, _),
+--   by_cases hp : p x,
+--   { simp only [hp, vector.to_list_cons, list.find_cons_of_pos, if_true,
+--       bind_const_dist_equiv_iff] },
+--   { simp only [hp, try_until, map_eq_bind_pure_comp, vector.to_list_cons,
+--       list.find_cons_of_neg, not_false_iff, if_false] }
+-- end
 
-/-- `oa.try_until p n` can fail to find a result iff there's an output `x` of `oa` with `¬ p x`. -/
-lemma none_mem_support_try_until_succ_iff :
-  none ∈ (oa.try_until p n.succ).support ↔ ∃ x ∈ oa.support, ¬ p x :=
-begin
-  simp only [try_until, mem_support_map_iff, list.find_eq_none],
-  exact ⟨λ h, let ⟨xs, hxs, hp⟩ := h in ⟨xs.head, mem_support_of_mem_of_support_repeat hxs
-    xs.head_mem, hp _ xs.head_mem⟩, λ h, let ⟨x, hx, hp⟩ := h in ⟨vector.replicate n.succ x,
-    replicate_mem_support_repeat n.succ hx, λ y hy, (list.eq_of_mem_replicate hy).symm ▸ hp⟩⟩
-end
+-- /-- `oa.try_until p n` can fail to find a result iff there's an output `x` of `oa` with `¬ p x`. -/
+-- lemma none_mem_support_try_until_succ_iff :
+--   none ∈ (oa.try_until p n.succ).support ↔ ∃ x ∈ oa.support, ¬ p x :=
+-- begin
+--   simp only [try_until, mem_support_map_iff, list.find_eq_none],
+--   exact ⟨λ h, let ⟨xs, hxs, hp⟩ := h in ⟨xs.head, mem_support_of_mem_of_support_repeat hxs
+--     xs.head_mem, hp _ xs.head_mem⟩, λ h, let ⟨x, hx, hp⟩ := h in ⟨vector.replicate n.succ x,
+--     replicate_mem_support_repeat n.succ hx, λ y hy, (list.eq_of_mem_replicate hy).symm ▸ hp⟩⟩
+-- end
 
-lemma none_mem_support_try_until_succ {x : α} (hx : x ∈ oa.support) (h : ¬ p x) :
-  none ∈ (oa.try_until p n.succ).support :=
-(none_mem_support_try_until_succ_iff oa p n).2 ⟨x, hx, h⟩
+-- lemma none_mem_support_try_until_succ {x : α} (hx : x ∈ oa.support) (h : ¬ p x) :
+--   none ∈ (oa.try_until p n.succ).support :=
+-- (none_mem_support_try_until_succ_iff oa p n).2 ⟨x, hx, h⟩
 
-lemma none_not_mem_support_try_until_succ (hx : ∀ x ∈ oa.support, p x) :
-  none ∉ (oa.try_until p n.succ).support :=
-mt (none_mem_support_try_until_succ_iff oa p n).1 (by simpa only [not_exists, not_not] using hx)
+-- lemma none_not_mem_support_try_until_succ (hx : ∀ x ∈ oa.support, p x) :
+--   none ∉ (oa.try_until p n.succ).support :=
+-- mt (none_mem_support_try_until_succ_iff oa p n).1 (by simpa only [not_exists, not_not] using hx)
 
-/-- The possible successful results of `oa.try_until p n` are outputs `x` of `oa` with `p x`. -/
-@[simp] lemma some_mem_support_try_until_succ_iff (x : α) :
-  some x ∈ (oa.try_until p n.succ).support ↔ x ∈ oa.support ∧ p x :=
-(mem_support_map_iff _ _ _).trans (⟨λ h, let ⟨xs, hxs, hp⟩ := h in
-  ⟨mem_support_of_mem_of_support_repeat hxs (list.find_mem hp), list.find_some hp⟩, λ h,
-    ⟨vector.replicate _ x, replicate_mem_support_repeat _ h.1, by simp [vector.replicate, h.2]⟩⟩)
+-- /-- The possible successful results of `oa.try_until p n` are outputs `x` of `oa` with `p x`. -/
+-- @[simp] lemma some_mem_support_try_until_succ_iff (x : α) :
+--   some x ∈ (oa.try_until p n.succ).support ↔ x ∈ oa.support ∧ p x :=
+-- (mem_support_map_iff _ _ _).trans (⟨λ h, let ⟨xs, hxs, hp⟩ := h in
+--   ⟨mem_support_of_mem_of_support_repeat hxs (list.find_mem hp), list.find_some hp⟩, λ h,
+--     ⟨vector.replicate _ x, replicate_mem_support_repeat _ h.1, by simp [vector.replicate, h.2]⟩⟩)
 
-lemma some_mem_support_try_until_succ {x : α} (hx : x ∈ oa.support) (h : p x) :
-  some x ∈ (oa.try_until p n.succ).support :=
-(some_mem_support_try_until_succ_iff oa p n x).2 ⟨hx, h⟩
+-- lemma some_mem_support_try_until_succ {x : α} (hx : x ∈ oa.support) (h : p x) :
+--   some x ∈ (oa.try_until p n.succ).support :=
+-- (some_mem_support_try_until_succ_iff oa p n x).2 ⟨hx, h⟩
 
-lemma some_not_mem_support_try_until_succ {x : α} (hx : x ∈ oa.support) (h : ¬ p x) :
-  some x ∉ (oa.try_until p n.succ).support :=
-λ h', false.elim (h ((some_mem_support_try_until_succ_iff _ _ _ _).1 h').2)
+-- lemma some_not_mem_support_try_until_succ {x : α} (hx : x ∈ oa.support) (h : ¬ p x) :
+--   some x ∉ (oa.try_until p n.succ).support :=
+-- λ h', false.elim (h ((some_mem_support_try_until_succ_iff _ _ _ _).1 h').2)
 
-/-- If at least one result of `oa` doesn't satisfy `p` then the result of `oa.try_until p n.succ`
-is either `none` (in the case of failure) or `some x` for some output `x` of `oa` with `p x`. -/
-lemma support_try_until_succ_of_exists_neg (h : ∃ x ∈ oa.support, ¬ p x) :
-  (oa.try_until p n.succ).support = insert none (some '' {x | x ∈ oa.support ∧ p x}) :=
-begin
-  refine trans (try_until_succ_dist_equiv oa p n).support_eq _,
-  rw [support_bind_ite_const_right _ _ _ _ h],
-  obtain ⟨x, hx, hpx⟩ := h,
-  refine set.ext (λ y, _),
-  cases y with y,
-  { have : none ∈ (oa.try_until p n).support,
-    from (mem_support_map_iff _ _ _).2 ⟨vector.replicate n x, replicate_mem_support_repeat n hx,
-      list.find_eq_none.2 (λ x' hx', (list.mem_replicate.1 hx').2.symm ▸ hpx)⟩,
-    simp [this] },
-  { have : some y ∈ (oa.try_until p n).support → y ∈ oa.support ∧ p y,
-    from λ h, ⟨mem_support_of_some_mem_support_try_until _ _ h,
-      pos_of_some_mem_support_try_until _ _ h⟩,
-    simpa using this }
-end
+-- /-- If at least one result of `oa` doesn't satisfy `p` then the result of `oa.try_until p n.succ`
+-- is either `none` (in the case of failure) or `some x` for some output `x` of `oa` with `p x`. -/
+-- lemma support_try_until_succ_of_exists_neg (h : ∃ x ∈ oa.support, ¬ p x) :
+--   (oa.try_until p n.succ).support = insert none (some '' {x | x ∈ oa.support ∧ p x}) :=
+-- begin
+--   refine trans (try_until_succ_dist_equiv oa p n).support_eq _,
+--   rw [support_bind_ite_const_right _ _ _ _ h],
+--   obtain ⟨x, hx, hpx⟩ := h,
+--   refine set.ext (λ y, _),
+--   cases y with y,
+--   { have : none ∈ (oa.try_until p n).support,
+--     from (mem_support_map_iff _ _ _).2 ⟨vector.replicate n x, replicate_mem_support_repeat n hx,
+--       list.find_eq_none.2 (λ x' hx', (list.mem_replicate.1 hx').2.symm ▸ hpx)⟩,
+--     simp [this] },
+--   { have : some y ∈ (oa.try_until p n).support → y ∈ oa.support ∧ p y,
+--     from λ h, ⟨mem_support_of_some_mem_support_try_until _ _ h,
+--       pos_of_some_mem_support_try_until _ _ h⟩,
+--     simpa using this }
+-- end
 
-/-- If all results of `oa` satisfy `p`, then `oa.try_until p n.succ` will just return `some x`,
-for some `x ∈ oa.support`(in particular the result of the first of the `n.succ` runs). -/
-lemma support_try_until_succ_of_forall_pos (hp : ∀ x ∈ oa.support, p x) :
-  (oa.try_until p n.succ).support = some '' oa.support :=
-begin
-  refine set.ext (λ y, ⟨λ h, _, λ h, _⟩),
-  { cases y with y,
-    { exact false.elim (none_not_mem_support_try_until_succ oa p n hp h) },
-    { exact ⟨y, mem_support_of_some_mem_support_try_until oa p h, rfl⟩ } },
-  { exact let ⟨x, hx⟩ := h in hx.2 ▸ some_mem_support_try_until_succ oa p _ hx.1 (hp x hx.1) }
-end
+-- /-- If all results of `oa` satisfy `p`, then `oa.try_until p n.succ` will just return `some x`,
+-- for some `x ∈ oa.support`(in particular the result of the first of the `n.succ` runs). -/
+-- lemma support_try_until_succ_of_forall_pos (hp : ∀ x ∈ oa.support, p x) :
+--   (oa.try_until p n.succ).support = some '' oa.support :=
+-- begin
+--   refine set.ext (λ y, ⟨λ h, _, λ h, _⟩),
+--   { cases y with y,
+--     { exact false.elim (none_not_mem_support_try_until_succ oa p n hp h) },
+--     { exact ⟨y, mem_support_of_some_mem_support_try_until oa p h, rfl⟩ } },
+--   { exact let ⟨x, hx⟩ := h in hx.2 ▸ some_mem_support_try_until_succ oa p _ hx.1 (hp x hx.1) }
+-- end
 
-end try_until_succ
+-- end try_until_succ
 
-section try_until_none
+-- section try_until_none
 
-/-- The probability of `oa.try_until p n` failing to generate a result is the probability
-of getting an output of `oa` not satisfying `p`, raised to the `n`th power. -/
-lemma prob_output_none_try_until : ⁅= none | oa.try_until p n⁆ = (1 - ⁅p | oa⁆) ^ n :=
-begin
-  induction n with n hn,
-  { rw [pow_zero, prob_output_try_until_zero] },
-  { refine ((try_until_succ_dist_equiv _ _ n).prob_output_eq none).trans _,
-    simp only [prob_output.def, prob_output_bind_ite_const_right, hn, ← pow_succ, eval_dist_return,
-      pmf.pure_apply, if_false, mul_zero, if_t_t, tsum_zero, zero_add] }
-end
+-- /-- The probability of `oa.try_until p n` failing to generate a result is the probability
+-- of getting an output of `oa` not satisfying `p`, raised to the `n`th power. -/
+-- lemma prob_output_none_try_until : ⁅= none | oa.try_until p n⁆ = (1 - ⁅p | oa⁆) ^ n :=
+-- begin
+--   induction n with n hn,
+--   { rw [pow_zero, prob_output_try_until_zero] },
+--   { refine ((try_until_succ_dist_equiv _ _ n).prob_output_eq none).trans _,
+--     simp only [prob_output.def, prob_output_bind_ite_const_right, hn, ← pow_succ, eval_dist_return,
+--       pmf.pure_apply, if_false, mul_zero, if_t_t, tsum_zero, zero_add] }
+-- end
 
-lemma prob_event_is_none_try_unitl :
-  ⁅λ x, x.is_none | oa.try_until p n⁆ = (1 - ⁅p | oa⁆) ^ n :=
-by rw [prob_event_is_none, prob_output_none_try_until]
+-- lemma prob_event_is_none_try_unitl :
+--   ⁅λ x, x.is_none | oa.try_until p n⁆ = (1 - ⁅p | oa⁆) ^ n :=
+-- by rw [prob_event_is_none, prob_output_none_try_until]
 
-end try_until_none
+-- end try_until_none
 
-section try_until_some
+-- section try_until_some
 
-lemma prob_event_is_some_try_until :
-  ⁅λ x, x.is_some | oa.try_until p n⁆ = 1 - (1 - ⁅p | oa⁆) ^ n :=
-by rw [prob_event_is_some_eq_one_sub_prob_output_none, prob_output_none_try_until]
+-- lemma prob_event_is_some_try_until :
+--   ⁅λ x, x.is_some | oa.try_until p n⁆ = 1 - (1 - ⁅p | oa⁆) ^ n :=
+-- by rw [prob_event_is_some_eq_one_sub_prob_output_none, prob_output_none_try_until]
 
-end try_until_some
+-- end try_until_some
 
-end oracle_comp
+-- end oracle_comp
